parameterize core defs with grammar symbol types

Defs.v
@@ -1,227 +1,241 @@
 Require Import FMaps List MSets Omega PeanoNat String.
 Require Import GallStar.Tactics.
 Require Import GallStar.Utils.
-        Import ListNotations.
+Import ListNotations.
 
-(* CORE PROJECT DEFINITIONS *)
+(* Types of grammar symbols; the user provides these at grammar definition time *)
+Module Type SYMBOL_TYPES.
 
-(* Representations of grammar symbols *)
-Definition terminal    := string.
-Definition nonterminal := nat.
-Inductive symbol       := T  : terminal -> symbol 
-                        | NT : nonterminal -> symbol.
+  Parameters terminal nonterminal : Type.
+  
+  Hypothesis t_eq_dec : forall a a' : terminal,
+      {a = a'} + {a <> a'}.
+  
+  Hypothesis nt_eq_dec : forall x x' : nonterminal,
+      {x = x'} + {x <> x'}.
 
-Lemma t_eq_dec :
-  forall a a' : terminal,
-    {a = a'} + {a <> a'}.
-Proof. repeat decide equality. Defined.
+  Parameter showT  : terminal    -> string.
+  Parameter showNT : nonterminal -> string.
+  
+End SYMBOL_TYPES.
 
-Lemma nt_eq_dec :
-  forall x x' : nonterminal,
-    {x = x'} + {x <> x'}.
-Proof. decide equality. Defined.
+(* Core definitions, parameterized by grammar symbol types *)
+Module DefsFn (Import Ty : SYMBOL_TYPES).
 
-Lemma gamma_eq_dec :
-  forall gamma gamma' : list symbol,
-    {gamma = gamma'} + {gamma <> gamma'}.
-Proof. repeat decide equality. Defined.
+  Inductive symbol       := T  : terminal -> symbol 
+                          | NT : nonterminal -> symbol.
 
-Definition beqGamma (xs ys : list symbol) : bool :=
-  if gamma_eq_dec xs ys then true else false.
+  Lemma symbol_eq_dec : forall s s' : symbol,
+      {s = s'} + {s <> s'}.
+  Proof. 
+    decide equality.
+    - apply Ty.t_eq_dec. 
+    - apply Ty.nt_eq_dec.
+  Defined.
 
-(* Finite sets of nonterminals *)
-Module MDT_NT.
-  Definition t      := nonterminal.
-  Definition eq_dec := Nat.eq_dec.
-End MDT_NT.
-Module NT_as_DT     := Make_UDT(MDT_NT).
-Module NtSet        := MSetWeakList.Make NT_as_DT.
-Module Export NF    := WFactsOn NT_as_DT NtSet.
-Module Export NP    := MSetProperties.Properties NtSet.
-Module Export NE    := EqProperties NtSet.
-Module Export ND    := WDecideOn NT_as_DT NtSet.
+  Lemma gamma_eq_dec :
+    forall gamma gamma' : list symbol,
+      {gamma = gamma'} + {gamma <> gamma'}.
+  Proof. 
+    decide equality. apply symbol_eq_dec. 
+  Defined.
 
-(* Hide an alternative definition of "sum" from NtSet *)
-Definition sum := Datatypes.sum.
+  Definition beqGamma (xs ys : list symbol) : bool :=
+    if gamma_eq_dec xs ys then true else false.
 
-(* Grammar-related definitions *)               
-Definition production := (nonterminal * list symbol)%type.
+  (* Finite sets of nonterminals *)
+  Module MDT_NT.
+    Definition t      := nonterminal.
+    Definition eq_dec := Ty.nt_eq_dec.
+  End MDT_NT.
+  Module NT_as_DT     := Make_UDT(MDT_NT).
+  Module NtSet        := MSetWeakList.Make NT_as_DT.
+  Module Export NF    := WFactsOn NT_as_DT NtSet.
+  Module Export NP    := MSetProperties.Properties NtSet.
+  Module Export NE    := EqProperties NtSet.
+  Module Export ND    := WDecideOn NT_as_DT NtSet.
 
-Definition grammar    := list production.
+  (* Hide an alternative definition of "sum" from NtSet *)
+  Definition sum := Datatypes.sum.
 
-Definition lhs (p : production) : nonterminal :=
-  let (x, _) := p in x.
+  (* Grammar-related definitions *)               
+  Definition production := (nonterminal * list symbol)%type.
 
-Definition lhss (g : grammar) : list nonterminal :=
-  map lhs g.
+  Definition grammar    := list production.
 
-Lemma production_lhs_in_lhss :
-  forall g x ys,
-    In (x, ys) g
-    -> In x (lhss g).
-Proof.
-  intros g x ys hi; induction g as [| (x', ys') ps IH]; sis.
-  - inv hi.
-  - destruct hi as [hh | ht].
-    + inv hh; apply in_eq.
-    + apply in_cons; auto.
-Qed.
+  Definition lhs (p : production) : nonterminal :=
+    let (x, _) := p in x.
 
-Definition rhs (p : production) : list symbol :=
-  let (_, gamma) := p in gamma.
+  Definition lhss (g : grammar) : list nonterminal :=
+    map lhs g.
 
-Definition rhss (g : grammar) : list (list symbol) :=
-  map rhs g.
+  Lemma production_lhs_in_lhss :
+    forall g x ys,
+      In (x, ys) g
+      -> In x (lhss g).
+  Proof.
+    intros g x ys hi; induction g as [| (x', ys') ps IH]; sis.
+    - inv hi.
+    - destruct hi as [hh | ht].
+      + inv hh; apply in_eq.
+      + apply in_cons; auto.
+  Qed.
 
-Fixpoint rhssForNt (ps : list production) (x : nonterminal) : list (list symbol) :=
-  match ps with
-  | []                 => []
-  | (x', gamma) :: ps' => 
-    if nt_eq_dec x' x then 
-      gamma :: rhssForNt ps' x
-    else 
-      rhssForNt ps' x
-  end.
+  Definition rhs (p : production) : list symbol :=
+    let (_, gamma) := p in gamma.
 
-Lemma rhssForNt_in_iff :
-  forall g x ys,
-    In ys (rhssForNt g x)
-    <-> In (x, ys) g.
-Proof.
-  intros g x ys; split; intros hi.
-  - induction g as [| (x', ys') g]; sis; tc.
-    destruct (nt_eq_dec x' x); subst; auto.
-    inv hi; auto.
-  - induction g as [| (x', ys') g]; sis; tc.
-    destruct hi as [heq | hi].
-    + inv heq.
-      destruct (nt_eq_dec x x); tc.
-      apply in_eq.
-    + destruct (nt_eq_dec x' x); subst; auto.
-      apply in_cons; auto.
-Qed.
-Hint Resolve rhssForNt_in_iff.
+  Definition rhss (g : grammar) : list (list symbol) :=
+    map rhs g.
 
-Lemma rhssForNt_rhss :
-  forall g x rhs,
-    In rhs (rhssForNt g x) -> In rhs (rhss g).
-Proof.
-  intros g x rhs Hin; induction g as [| (x', rhs') ps IH]; simpl in *.
-  - inv Hin.
-  - destruct (nt_eq_dec x' x); subst; auto.
-    destruct Hin as [Heq | Hin]; subst; auto.
-Qed.
+  Fixpoint rhssForNt (ps : list production) (x : nonterminal) : list (list symbol) :=
+    match ps with
+    | []                 => []
+    | (x', gamma) :: ps' => 
+      if Ty.nt_eq_dec x' x then 
+        gamma :: rhssForNt ps' x
+      else 
+        rhssForNt ps' x
+    end.
 
-Definition rhsLengths (g : grammar) : list nat :=
-  map (fun rhs => List.length rhs) (rhss g).
+  Lemma rhssForNt_in_iff :
+    forall g x ys,
+      In ys (rhssForNt g x)
+      <-> In (x, ys) g.
+  Proof.
+    intros g x ys; split; intros hi.
+    - induction g as [| (x', ys') g]; sis; tc.
+      destruct (Ty.nt_eq_dec x' x); subst; auto.
+      inv hi; auto.
+    - induction g as [| (x', ys') g]; sis; tc.
+      destruct hi as [heq | hi].
+      + inv heq.
+        destruct (Ty.nt_eq_dec x x); tc.
+        apply in_eq.
+      + destruct (Ty.nt_eq_dec x' x); subst; auto.
+        apply in_cons; auto.
+  Qed.
+  Hint Resolve rhssForNt_in_iff.
 
-Lemma rhss_rhsLengths_in :
-  forall g rhs,
-    In rhs (rhss g)
-    -> In (List.length rhs) (rhsLengths g).
-Proof.
-  intros g rhs Hin; induction g as [| (x, rhs') ps IH];
-  simpl in *; inv Hin; auto.
-Qed.
+  Lemma rhssForNt_rhss :
+    forall g x rhs,
+      In rhs (rhssForNt g x) -> In rhs (rhss g).
+  Proof.
+    intros g x rhs Hin; induction g as [| (x', rhs') ps IH]; simpl in *.
+    - inv Hin.
+    - destruct (Ty.nt_eq_dec x' x); subst; auto.
+      destruct Hin as [Heq | Hin]; subst; auto.
+  Qed.
 
-Definition maxRhsLength (g : grammar) : nat :=
-  listMax (rhsLengths g).
+  Definition rhsLengths (g : grammar) : list nat :=
+    map (fun rhs => List.length rhs) (rhss g).
 
-Lemma grammar_rhs_length_le_max :
-  forall g x rhs,
-    In (x, rhs) g
-    -> List.length rhs <= maxRhsLength g.
-Proof.
-  intros; unfold maxRhsLength.
-  apply listMax_in_le.
-  apply rhss_rhsLengths_in.
-  eapply rhssForNt_rhss.
-  eapply rhssForNt_in_iff; eauto.
-Qed.
+  Lemma rhss_rhsLengths_in :
+    forall g rhs,
+      In rhs (rhss g)
+      -> In (List.length rhs) (rhsLengths g).
+  Proof.
+    intros g rhs Hin; induction g as [| (x, rhs') ps IH];
+      simpl in *; inv Hin; auto.
+  Qed.
 
-Lemma grammar_rhs_length_lt_max_plus_1 :
-  forall g x rhs,
-    In (x, rhs) g
-    -> List.length rhs < 1 + maxRhsLength g.
-Proof.
-  intros g x rhs Hin.
-  apply grammar_rhs_length_le_max in Hin; omega.
-Qed.
+  Definition maxRhsLength (g : grammar) : nat :=
+    listMax (rhsLengths g).
 
-Definition fromNtList (ls : list nonterminal) : NtSet.t :=
-  fold_right NtSet.add NtSet.empty ls.
+  Lemma grammar_rhs_length_le_max :
+    forall g x rhs,
+      In (x, rhs) g
+      -> List.length rhs <= maxRhsLength g.
+  Proof.
+    intros; unfold maxRhsLength.
+    apply listMax_in_le.
+    apply rhss_rhsLengths_in.
+    eapply rhssForNt_rhss.
+    eapply rhssForNt_in_iff; eauto.
+  Qed.
 
-Lemma fromNtList_in_iff :
-  forall (x : nonterminal)
-         (l : list nonterminal), 
-    In x l <-> NtSet.In x (fromNtList l).
-Proof.
-  intros x l; split; intro hi; induction l as [| x' l IH]; sis; try ND.fsetdec.
-  - destruct hi as [hh | ht]; subst; auto.
-    + ND.fsetdec.
-    + apply IH in ht; ND.fsetdec.
-  - destruct (NF.eq_dec x' x); subst; auto.
-    right; apply IH; ND.fsetdec.
-Qed.
+  Lemma grammar_rhs_length_lt_max_plus_1 :
+    forall g x rhs,
+      In (x, rhs) g
+      -> List.length rhs < 1 + maxRhsLength g.
+  Proof.
+    intros g x rhs Hin.
+    apply grammar_rhs_length_le_max in Hin; omega.
+  Qed.
 
-Definition allNts (g : grammar) : NtSet.t := 
-  fromNtList (lhss g).
+  Definition fromNtList (ls : list nonterminal) : NtSet.t :=
+    fold_right NtSet.add NtSet.empty ls.
 
-Lemma allNts_lhss_iff :
-  forall (g : grammar) (x : nonterminal),
-    In x (lhss g)
-    <-> NtSet.In x (allNts g).
-Proof.
-  intros g x; split; intros hi; apply fromNtList_in_iff; auto.
-Qed.
+  Lemma fromNtList_in_iff :
+    forall (x : nonterminal)
+           (l : list nonterminal), 
+      In x l <-> NtSet.In x (fromNtList l).
+  Proof.
+    intros x l; split; intro hi; induction l as [| x' l IH]; sis; try ND.fsetdec.
+    - destruct hi as [hh | ht]; subst; auto.
+      + ND.fsetdec.
+      + apply IH in ht; ND.fsetdec.
+    - destruct (NF.eq_dec x' x); subst; auto.
+      right; apply IH; ND.fsetdec.
+  Qed.
 
-Lemma lhs_mem_allNts_true :
-  forall g x ys,
-    In (x, ys) g
-    -> NtSet.mem x (allNts g) = true.
-Proof.
-  intros g x ys hi.
-  apply NtSet.mem_spec.
-  apply allNts_lhss_iff. 
-  eapply production_lhs_in_lhss; eauto.
-Qed.
+  Definition allNts (g : grammar) : NtSet.t := 
+    fromNtList (lhss g).
 
-(* Definitions related to input that the parser consumes. *)
-Definition literal := string.
+  Lemma allNts_lhss_iff :
+    forall (g : grammar) (x : nonterminal),
+      In x (lhss g)
+      <-> NtSet.In x (allNts g).
+  Proof.
+    intros g x; split; intros hi; apply fromNtList_in_iff; auto.
+  Qed.
 
-Definition token   := (terminal * literal)% type.
+  Lemma lhs_mem_allNts_true :
+    forall g x ys,
+      In (x, ys) g
+      -> NtSet.mem x (allNts g) = true.
+  Proof.
+    intros g x ys hi.
+    apply NtSet.mem_spec.
+    apply allNts_lhss_iff. 
+    eapply production_lhs_in_lhss; eauto.
+  Qed.
 
-(* Parser return values *)
-Inductive tree    := Leaf : terminal -> literal -> tree
-                   | Node : nonterminal -> list tree -> tree.
+  (* Definitions related to input that the parser consumes. *)
+  Definition literal := string.
 
-Definition forest := list tree.
+  Definition token   := (terminal * literal)% type.
 
-(* Parser stacks *)
-Inductive prefix_frame :=
-| PF : list symbol -> forest -> prefix_frame.
+  (* Parser return values *)
+  Inductive tree    := Leaf : terminal -> literal -> tree
+                     | Node : nonterminal -> list tree -> tree.
 
-Definition prefix_stack := (prefix_frame * list prefix_frame)%type.
+  Definition forest := list tree.
 
-Inductive suffix_frame :=
-| SF : list symbol -> suffix_frame.
+  (* Parser stacks *)
+  Inductive prefix_frame :=
+  | PF : list symbol -> forest -> prefix_frame.
 
-Definition suffix_stack := (suffix_frame * list suffix_frame)%type. 
+  Definition prefix_stack := (prefix_frame * list prefix_frame)%type.
 
-Fixpoint unprocTailSyms (frs : list suffix_frame) : list symbol :=
-  match frs with 
-  | []                        => []
-  | SF [] :: _               => [] (* impossible for a well-formed stack *)
-  | SF (T _ :: _) :: _       => [] (* impossible for a well-formed stack *)
-  | SF (NT x :: suf) :: frs' => suf ++ unprocTailSyms frs'
-  end.
+  Inductive suffix_frame :=
+  | SF : list symbol -> suffix_frame.
 
-Definition unprocStackSyms (stk : suffix_stack) : list symbol :=
-  match stk with
-  | (SF suf, frs) => suf ++ unprocTailSyms frs
-  end.
+  Definition suffix_stack := (suffix_frame * list suffix_frame)%type. 
 
-(*
+  Fixpoint unprocTailSyms (frs : list suffix_frame) : list symbol :=
+    match frs with 
+    | []                        => []
+    | SF [] :: _               => [] (* impossible for a well-formed stack *)
+    | SF (T _ :: _) :: _       => [] (* impossible for a well-formed stack *)
+    | SF (NT x :: suf) :: frs' => suf ++ unprocTailSyms frs'
+    end.
+
+  Definition unprocStackSyms (stk : suffix_stack) : list symbol :=
+    match stk with
+    | (SF suf, frs) => suf ++ unprocTailSyms frs
+    end.
+
+  (*
 Definition bottomFramePrefix (p_stk : prefix_stack) : list symbol :=
   match bottomElt p_stk with
   | PF pre _ => pre
@@ -231,389 +245,401 @@ Definition bottomFrameSuffix (s_stk : suffix_stack) : list symbol :=
   match bottomElt s_stk with
   | SF suf => suf
   end.
-*)
-Definition bottomFrameSyms p_stk s_stk := 
-  match bottomElt p_stk, bottomElt s_stk with
-  | PF pre _, SF suf => rev pre ++ suf
-  end.
+   *)
+  Definition bottomFrameSyms p_stk s_stk := 
+    match bottomElt p_stk, bottomElt s_stk with
+    | PF pre _, SF suf => rev pre ++ suf
+    end.
 
-(* Grammatical derivation relation *)
-Inductive sym_derivation (g : grammar) : symbol -> list token -> tree -> Prop :=
-| T_der  : 
-    forall (a : terminal) (l : literal),
-      sym_derivation g (T a) [(a, l)] (Leaf a l)
-| NT_der : 
-    forall (x  : nonterminal) (ys : list symbol) (w : list token) (sts : forest),
-      In (x, ys) g
-      -> gamma_derivation g ys w sts
-      -> sym_derivation g (NT x) w (Node x sts)
-with gamma_derivation (g : grammar) : list symbol -> list token-> forest-> Prop :=
-     | Nil_der  : 
-         gamma_derivation g [] [] []
-     | Cons_der : 
-         forall (s : symbol) (ss : list symbol) (wpre wsuf : list token) 
-                (tr : tree) (trs : list tree),
-           sym_derivation g s wpre tr
-           -> gamma_derivation g ss wsuf trs
-           -> gamma_derivation g (s :: ss) (wpre ++ wsuf) (tr :: trs).
+  (* Grammatical derivation relation *)
+  Inductive sym_derivation (g : grammar) : symbol -> list token -> tree -> Prop :=
+  | T_der  : 
+      forall (a : terminal) (l : literal),
+        sym_derivation g (T a) [(a, l)] (Leaf a l)
+  | NT_der : 
+      forall (x  : nonterminal) (ys : list symbol) (w : list token) (sts : forest),
+        In (x, ys) g
+        -> gamma_derivation g ys w sts
+        -> sym_derivation g (NT x) w (Node x sts)
+  with gamma_derivation (g : grammar) : list symbol -> list token-> forest-> Prop :=
+       | Nil_der  : 
+           gamma_derivation g [] [] []
+       | Cons_der : 
+           forall (s : symbol) (ss : list symbol) (wpre wsuf : list token) 
+                  (tr : tree) (trs : list tree),
+             sym_derivation g s wpre tr
+             -> gamma_derivation g ss wsuf trs
+             -> gamma_derivation g (s :: ss) (wpre ++ wsuf) (tr :: trs).
 
-Hint Constructors sym_derivation gamma_derivation.
+  Hint Constructors sym_derivation gamma_derivation.
 
-Scheme sym_derivation_mutual_ind   := Induction for sym_derivation Sort Prop
-  with gamma_derivation_mutual_ind := Induction for gamma_derivation Sort Prop.
+  Scheme sym_derivation_mutual_ind   := Induction for sym_derivation Sort Prop
+    with gamma_derivation_mutual_ind := Induction for gamma_derivation Sort Prop.
 
-Ltac inv_sd hs  hi hg:=
-  inversion hs as [ ? ? | ? ? ? ? hi hg]; subst; clear hs.
+  Ltac inv_sd hs  hi hg:=
+    inversion hs as [ ? ? | ? ? ? ? hi hg]; subst; clear hs.
 
-Ltac inv_gd hg  hs hg' :=
-  inversion hg as [| ? ? ? ? ? ? hs hg']; subst; clear hg.
+  Ltac inv_gd hg  hs hg' :=
+    inversion hg as [| ? ? ? ? ? ? hs hg']; subst; clear hg.
 
-Lemma gamma_derivation_app' :
-  forall g ys1 w1 v1,
-    gamma_derivation g ys1 w1 v1
-    -> forall ys2 w2 v2,
-      gamma_derivation g ys2 w2 v2
-      -> gamma_derivation g (ys1 ++ ys2) (w1 ++ w2) (v1 ++ v2).
-Proof.
-  intros g ys1 w1 v1 hg.
-  induction hg; intros ys2 w2 v2 hg2; simpl in *; auto.
-  rewrite <- app_assoc; constructor; auto.
-Qed.
+  Lemma gamma_derivation_app' :
+    forall g ys1 w1 v1,
+      gamma_derivation g ys1 w1 v1
+      -> forall ys2 w2 v2,
+        gamma_derivation g ys2 w2 v2
+        -> gamma_derivation g (ys1 ++ ys2) (w1 ++ w2) (v1 ++ v2).
+  Proof.
+    intros g ys1 w1 v1 hg.
+    induction hg; intros ys2 w2 v2 hg2; simpl in *; auto.
+    rewrite <- app_assoc; constructor; auto.
+  Qed.
 
-Lemma gamma_derivation_app :
-  forall g ys ys' w w' v v',
-    gamma_derivation g ys w v
-    -> gamma_derivation g ys' w' v'
-    -> gamma_derivation g (ys ++ ys') (w ++ w') (v ++ v').
-Proof.
-  intros; eapply gamma_derivation_app'; eauto.
-Qed.
+  Lemma gamma_derivation_app :
+    forall g ys ys' w w' v v',
+      gamma_derivation g ys w v
+      -> gamma_derivation g ys' w' v'
+      -> gamma_derivation g (ys ++ ys') (w ++ w') (v ++ v').
+  Proof.
+    intros; eapply gamma_derivation_app'; eauto.
+  Qed.
 
-Lemma forest_app_singleton_node : 
-  forall g x ys ys' w w' v v',
-    In (x, ys') g
-    -> gamma_derivation g ys w v
-    -> gamma_derivation g ys' w' v'
-    -> gamma_derivation g (ys ++ [NT x]) (w ++ w') (v ++ [Node x v']).
-Proof.
-  intros g x ys ys' w w' v v' hi hg hg'.
-  apply gamma_derivation_app; auto.
-  rew_nil_r w'; eauto.
-Qed.
+  Lemma forest_app_singleton_node : 
+    forall g x ys ys' w w' v v',
+      In (x, ys') g
+      -> gamma_derivation g ys w v
+      -> gamma_derivation g ys' w' v'
+      -> gamma_derivation g (ys ++ [NT x]) (w ++ w') (v ++ [Node x v']).
+  Proof.
+    intros g x ys ys' w w' v v' hi hg hg'.
+    apply gamma_derivation_app; auto.
+    rew_nil_r w'; eauto.
+  Qed.
 
-Lemma terminal_head_gamma_derivation :
-  forall g a l ys w v,
-    gamma_derivation g ys w v
-    -> gamma_derivation g (T a :: ys) ((a, l) :: w) (Leaf a l :: v).
-Proof.
-  intros g a l ys w v hg.
-  assert (happ : (a, l) :: w = [(a, l)] ++ w) by apply cons_app_singleton.
-  rewrite happ; auto.
-Qed.
+  Lemma terminal_head_gamma_derivation :
+    forall g a l ys w v,
+      gamma_derivation g ys w v
+      -> gamma_derivation g (T a :: ys) ((a, l) :: w) (Leaf a l :: v).
+  Proof.
+    intros g a l ys w v hg.
+    assert (happ : (a, l) :: w = [(a, l)] ++ w) by apply cons_app_singleton.
+    rewrite happ; auto.
+  Qed.
 
-Lemma gamma_derivation_split :
-  forall g ys ys' w'' v'',
-    gamma_derivation g (ys ++ ys') w'' v''
-    -> exists w w' v v',
-      w'' = w ++ w'
-      /\ v'' = v ++ v'
-      /\ gamma_derivation g ys  w  v
-      /\ gamma_derivation g ys' w' v'.
-Proof.
-  intros g ys; induction ys as [| y ys IH]; intros ys' w'' v'' hg; sis.
-  - exists []; exists w''; exists []; exists v''; repeat split; auto.
-  - inversion hg as [| s ss wpre wsuf t f hs hg']; subst; clear hg. 
-    apply IH in hg'; destruct hg' as [w [w' [v [v' [? [? [hg' hg'']]]]]]]; subst.
-    exists (wpre ++ w); exists w'; exists (t :: v); exists v'. 
-    repeat split; auto; apps.
-Qed.
+  Lemma gamma_derivation_split :
+    forall g ys ys' w'' v'',
+      gamma_derivation g (ys ++ ys') w'' v''
+      -> exists w w' v v',
+        w'' = w ++ w'
+        /\ v'' = v ++ v'
+        /\ gamma_derivation g ys  w  v
+        /\ gamma_derivation g ys' w' v'.
+  Proof.
+    intros g ys; induction ys as [| y ys IH]; intros ys' w'' v'' hg; sis.
+    - exists []; exists w''; exists []; exists v''; repeat split; auto.
+    - inversion hg as [| s ss wpre wsuf t f hs hg']; subst; clear hg. 
+      apply IH in hg'; destruct hg' as [w [w' [v [v' [? [? [hg' hg'']]]]]]]; subst.
+      exists (wpre ++ w); exists w'; exists (t :: v); exists v'. 
+      repeat split; auto; apps.
+  Qed.
 
-Lemma gamma_derivation_terminal_end :
-  forall g ys a w v,
-    gamma_derivation g (ys ++ [T a]) w v
-    -> exists w_front l v_front,
-      w = w_front ++ [(a, l)]
-      /\ v = v_front ++ [Leaf a l]
-      /\ gamma_derivation g ys w_front v_front.
-Proof.
-  intros g ys a w v hg.
-  eapply gamma_derivation_split in hg.
-  destruct hg as [w' [w'' [v' [v'' [? [? [hg hg']]]]]]]; subst.
-  inv hg'.
-  (* lemma *)
-  inv H1. inv H4.
-  repeat eexists; eauto.
-Qed.
+  Lemma gamma_derivation_terminal_end :
+    forall g ys a w v,
+      gamma_derivation g (ys ++ [T a]) w v
+      -> exists w_front l v_front,
+        w = w_front ++ [(a, l)]
+        /\ v = v_front ++ [Leaf a l]
+        /\ gamma_derivation g ys w_front v_front.
+  Proof.
+    intros g ys a w v hg.
+    eapply gamma_derivation_split in hg.
+    destruct hg as [w' [w'' [v' [v'' [? [? [hg hg']]]]]]]; subst.
+    inv hg'.
+    (* lemma *)
+    inv H1. inv H4.
+    repeat eexists; eauto.
+  Qed.
 
-Lemma gamma_derivation_nonterminal_end :
-  forall g ys x w v,
-    gamma_derivation g (ys ++ [NT x]) w v
-    -> exists wpre wsuf vpre v',
-      w = wpre ++ wsuf
-      /\ v = vpre ++ [Node x v']
-      /\ gamma_derivation g ys wpre vpre
-      /\ sym_derivation g (NT x) wsuf (Node x v').
-Proof.
-  intros g ys x w v hg.
-  eapply gamma_derivation_split in hg.
-  destruct hg as [w' [w'' [v' [v'' [? [? [hg hg']]]]]]]; subst.
-  inv hg'.
-  (* lemma *)
-  inv H4. rewrite app_nil_r in *.
-  inv H1.
-  repeat eexists; eauto.
-Qed.
+  Lemma gamma_derivation_nonterminal_end :
+    forall g ys x w v,
+      gamma_derivation g (ys ++ [NT x]) w v
+      -> exists wpre wsuf vpre v',
+        w = wpre ++ wsuf
+        /\ v = vpre ++ [Node x v']
+        /\ gamma_derivation g ys wpre vpre
+        /\ sym_derivation g (NT x) wsuf (Node x v').
+  Proof.
+    intros g ys x w v hg.
+    eapply gamma_derivation_split in hg.
+    destruct hg as [w' [w'' [v' [v'' [? [? [hg hg']]]]]]]; subst.
+    inv hg'.
+    (* lemma *)
+    inv H4. rewrite app_nil_r in *.
+    inv H1.
+    repeat eexists; eauto.
+  Qed.
 
-Lemma trees_eq__gammas_eq_words_eq' :
-  forall g ys w v,
-    gamma_derivation g ys w v
-    -> forall ys' w',
+  Lemma trees_eq__gammas_eq_words_eq' :
+    forall g ys w v,
+      gamma_derivation g ys w v
+      -> forall ys' w',
         gamma_derivation g ys' w' v
         -> ys' = ys /\ w' = w.
-Proof.
-  intros g ys w v hg.
-  induction hg using gamma_derivation_mutual_ind with
-      (P := fun s w t (hs : sym_derivation g s w t) =>
-              forall s' w',
-                sym_derivation g s' w' t
-                -> s' = s /\ w' = w).
-  - intros s' w' hs; inv hs; auto.
-  - intros s' w' hs; inv hs; firstorder.
-  - intros ys' w' hg; inv hg; auto.
-  - intros ys' w' hg'; inv hg'.
-    apply IHhg in H3; destruct H3; subst.
-    apply IHhg0 in H4; destruct H4; subst; auto.
-Qed.
+  Proof.
+    intros g ys w v hg.
+    induction hg using gamma_derivation_mutual_ind with
+        (P := fun s w t (hs : sym_derivation g s w t) =>
+                forall s' w',
+                  sym_derivation g s' w' t
+                  -> s' = s /\ w' = w).
+    - intros s' w' hs; inv hs; auto.
+    - intros s' w' hs; inv hs; firstorder.
+    - intros ys' w' hg; inv hg; auto.
+    - intros ys' w' hg'; inv hg'.
+      apply IHhg in H3; destruct H3; subst.
+      apply IHhg0 in H4; destruct H4; subst; auto.
+  Qed.
 
-Lemma trees_eq__gammas_eq_words_eq :
-  forall g ys ys' w w' v,
-    gamma_derivation g ys w v
-    -> gamma_derivation g ys' w' v
-    -> ys' = ys /\ w' = w.
-Proof.
-  intros; eapply trees_eq__gammas_eq_words_eq'; eauto.
-Qed.
+  Lemma trees_eq__gammas_eq_words_eq :
+    forall g ys ys' w w' v,
+      gamma_derivation g ys w v
+      -> gamma_derivation g ys' w' v
+      -> ys' = ys /\ w' = w.
+  Proof.
+    intros; eapply trees_eq__gammas_eq_words_eq'; eauto.
+  Qed.
 
-Lemma gamma_derivation_singleton_t :
-  forall g a w v,
-    gamma_derivation g [T a] w v
-    -> exists l,
-      w = [(a, l)]
-      /\ v = [Leaf a l].
-Proof.
-  intros g a w v hg.
-  inv_gd hg hs hg'.
-  inv hs; inv hg'; rewrite app_nil_r; eauto.
-Qed.
+  Lemma gamma_derivation_singleton_t :
+    forall g a w v,
+      gamma_derivation g [T a] w v
+      -> exists l,
+        w = [(a, l)]
+        /\ v = [Leaf a l].
+  Proof.
+    intros g a w v hg.
+    inv_gd hg hs hg'.
+    inv hs; inv hg'; rewrite app_nil_r; eauto.
+  Qed.
 
-Lemma gamma_derivation_singleton_nt :
-  forall g x w v,
-    gamma_derivation g [NT x] w v
-    -> exists ys v',
-      In (x, ys) g
-      /\ v = [Node x v']
-      /\ gamma_derivation g ys w v'.
-Proof.
-  intros g x w v hg.
-  inv_gd hg hs hg'.
-  inv hs; inv hg'; rewrite app_nil_r; eauto.
-Qed.
+  Lemma gamma_derivation_singleton_nt :
+    forall g x w v,
+      gamma_derivation g [NT x] w v
+      -> exists ys v',
+        In (x, ys) g
+        /\ v = [Node x v']
+        /\ gamma_derivation g ys w v'.
+  Proof.
+    intros g x w v hg.
+    inv_gd hg hs hg'.
+    inv hs; inv hg'; rewrite app_nil_r; eauto.
+  Qed.
 
-Definition unique_gamma_derivation g ss w v :=
-  gamma_derivation g ss w v
-  /\ forall v', gamma_derivation g ss w v' -> v = v'.
+  Definition unique_gamma_derivation g ss w v :=
+    gamma_derivation g ss w v
+    /\ forall v', gamma_derivation g ss w v' -> v = v'.
 
-Inductive sym_recognize (g : grammar) : symbol -> list token -> Prop :=
-| T_rec  : 
-    forall (a : terminal) (l : literal),
-      sym_recognize g (T a) [(a, l)]
-| NT_rec : 
-    forall (x  : nonterminal) (ys : list symbol) (w : list token),
-      In (x, ys) g
-      -> gamma_recognize g ys w
-      -> sym_recognize g (NT x) w
-with gamma_recognize (g : grammar) : list symbol -> list token -> Prop :=
-     | Nil_rec  : 
-         gamma_recognize g [] []
-     | Cons_rec : 
-         forall (s : symbol) (ss : list symbol) (wpre wsuf : list token),
-           sym_recognize g s wpre
-           -> gamma_recognize g ss wsuf
-           -> gamma_recognize g (s :: ss) (wpre ++ wsuf).
+  Inductive sym_recognize (g : grammar) : symbol -> list token -> Prop :=
+  | T_rec  : 
+      forall (a : terminal) (l : literal),
+        sym_recognize g (T a) [(a, l)]
+  | NT_rec : 
+      forall (x  : nonterminal) (ys : list symbol) (w : list token),
+        In (x, ys) g
+        -> gamma_recognize g ys w
+        -> sym_recognize g (NT x) w
+  with gamma_recognize (g : grammar) : list symbol -> list token -> Prop :=
+       | Nil_rec  : 
+           gamma_recognize g [] []
+       | Cons_rec : 
+           forall (s : symbol) (ss : list symbol) (wpre wsuf : list token),
+             sym_recognize g s wpre
+             -> gamma_recognize g ss wsuf
+             -> gamma_recognize g (s :: ss) (wpre ++ wsuf).
 
-Hint Constructors sym_recognize gamma_recognize.
+  Hint Constructors sym_recognize gamma_recognize.
 
-Ltac inv_sr hs  hi hg :=
-  inversion hs as [ ? ? | ? ? ? hi hg ]; subst; clear hs.
+  Ltac inv_sr hs  hi hg :=
+    inversion hs as [ ? ? | ? ? ? hi hg ]; subst; clear hs.
 
-Ltac inv_gr hg  wpre wsuf hs hg' :=
-  inversion hg as [| ? ? wpre wsuf hs hg']; subst; clear hg.
+  Ltac inv_gr hg  wpre wsuf hs hg' :=
+    inversion hg as [| ? ? wpre wsuf hs hg']; subst; clear hg.
 
-Scheme sym_recognize_mutual_ind   := Induction for sym_recognize Sort Prop
-  with gamma_recognize_mutual_ind := Induction for gamma_recognize Sort Prop.
+  Scheme sym_recognize_mutual_ind   := Induction for sym_recognize Sort Prop
+    with gamma_recognize_mutual_ind := Induction for gamma_recognize Sort Prop.
 
-Lemma gamma_recognize_terminal_head :
-  forall g a suf w,
-    gamma_recognize g (T a :: suf) w
-    -> exists l w',
-      w = (a, l) :: w'
-      /\ gamma_recognize g suf w'.
-Proof.
-  intros g a suf w hg.
-  inversion hg as [| h t wpre wsuf hs hg']; subst; clear hg.
-  inv hs; simpl; eauto.
-Qed.
+  Lemma gamma_recognize_terminal_head :
+    forall g a suf w,
+      gamma_recognize g (T a :: suf) w
+      -> exists l w',
+        w = (a, l) :: w'
+        /\ gamma_recognize g suf w'.
+  Proof.
+    intros g a suf w hg.
+    inversion hg as [| h t wpre wsuf hs hg']; subst; clear hg.
+    inv hs; simpl; eauto.
+  Qed.
 
-Lemma gamma_recognize_nonterminal_head :
-  forall g x suf w,
-    gamma_recognize g (NT x :: suf) w
-    -> exists rhs wpre wsuf,
-      w = wpre ++ wsuf
-      /\ In (x, rhs) g
-      /\ gamma_recognize g rhs wpre
-      /\ gamma_recognize g suf wsuf.
-Proof.
-  intros g x suf w hg.
-  inversion hg as [| h t wpre wsuf hs hg']; subst; clear hg.
-  inv hs; simpl; eauto 8.
-Qed.
+  Lemma gamma_recognize_nonterminal_head :
+    forall g x suf w,
+      gamma_recognize g (NT x :: suf) w
+      -> exists rhs wpre wsuf,
+        w = wpre ++ wsuf
+        /\ In (x, rhs) g
+        /\ gamma_recognize g rhs wpre
+        /\ gamma_recognize g suf wsuf.
+  Proof.
+    intros g x suf w hg.
+    inversion hg as [| h t wpre wsuf hs hg']; subst; clear hg.
+    inv hs; simpl; eauto 8.
+  Qed.
 
-Lemma gamma_recognize_app' :
-  forall g ys1 w1,
-    gamma_recognize g ys1 w1
-    -> forall ys2 w2,
-      gamma_recognize g ys2 w2
+  Lemma gamma_recognize_app' :
+    forall g ys1 w1,
+      gamma_recognize g ys1 w1
+      -> forall ys2 w2,
+        gamma_recognize g ys2 w2
+        -> gamma_recognize g (ys1 ++ ys2) (w1 ++ w2).
+  Proof.
+    intros g ys1 w1 hg.
+    induction hg; intros ys2 w2 hg2; simpl in *; auto.
+    rewrite <- app_assoc; constructor; auto.
+  Qed.
+
+  Lemma gamma_recognize_app :
+    forall g ys1 ys2 w1 w2,
+      gamma_recognize g ys1 w1
+      -> gamma_recognize g ys2 w2
       -> gamma_recognize g (ys1 ++ ys2) (w1 ++ w2).
-Proof.
-  intros g ys1 w1 hg.
-  induction hg; intros ys2 w2 hg2; simpl in *; auto.
-  rewrite <- app_assoc; constructor; auto.
-Qed.
+  Proof.
+    intros; apply gamma_recognize_app'; auto.
+  Qed.
 
-Lemma gamma_recognize_app :
-  forall g ys1 ys2 w1 w2,
-    gamma_recognize g ys1 w1
-    -> gamma_recognize g ys2 w2
-    -> gamma_recognize g (ys1 ++ ys2) (w1 ++ w2).
-Proof.
-  intros; apply gamma_recognize_app'; auto.
-Qed.
+  Lemma gamma_recognize_split :
+    forall g ys ys' w'',
+      gamma_recognize g (ys ++ ys') w''
+      -> exists w w',
+        w'' = w ++ w'
+        /\ gamma_recognize g ys w
+        /\ gamma_recognize g ys' w'.
+  Proof.
+    intros g ys; induction ys as [| y ys IH]; intros ys' w'' hg; sis.
+    - exists []; exists w''; repeat split; auto.
+    - inversion hg as [| s ss wpre wsuf hs hg']; subst; clear hg. 
+      apply IH in hg'; destruct hg' as [w [w' [? [hg' hg'']]]]; subst.
+      exists (wpre ++ w); exists w'; repeat split; auto; apps.
+  Qed.
 
-Lemma gamma_recognize_split :
-  forall g ys ys' w'',
-    gamma_recognize g (ys ++ ys') w''
-    -> exists w w',
-      w'' = w ++ w'
-      /\ gamma_recognize g ys w
-      /\ gamma_recognize g ys' w'.
-Proof.
-  intros g ys; induction ys as [| y ys IH]; intros ys' w'' hg; sis.
-  - exists []; exists w''; repeat split; auto.
-  - inversion hg as [| s ss wpre wsuf hs hg']; subst; clear hg. 
-    apply IH in hg'; destruct hg' as [w [w' [? [hg' hg'']]]]; subst.
-    exists (wpre ++ w); exists w'; repeat split; auto; apps.
-Qed.
+  Lemma gamma_derivation__gamma_recognize :
+    forall g ys w v,
+      gamma_derivation g ys w v
+      -> gamma_recognize g ys w.
+  Proof.
+    intros g ys w v hg.
+    induction hg using gamma_derivation_mutual_ind with
+        (P := fun s w t (hs : sym_derivation g s w t) => 
+                sym_recognize g s w); eauto.
+  Qed.
 
-Lemma gamma_derivation__gamma_recognize :
-  forall g ys w v,
-    gamma_derivation g ys w v
-    -> gamma_recognize g ys w.
-Proof.
-  intros g ys w v hg.
-  induction hg using gamma_derivation_mutual_ind with
-      (P := fun s w t (hs : sym_derivation g s w t) => 
-              sym_recognize g s w); eauto.
-Qed.
+  Lemma gamma_recognize__exists_gamma_derivation :
+    forall g ys w,
+      gamma_recognize g ys w
+      -> exists v,
+        gamma_derivation g ys w v.
+  Proof.
+    intros g ys w hg.
+    induction hg using gamma_recognize_mutual_ind with
+        (P := fun s w (hs : sym_recognize g s w) => 
+                exists t, sym_derivation g s w t); firstorder; eauto.
+    repeat econstructor; eauto.
+  Qed.
 
-Lemma gamma_recognize__exists_gamma_derivation :
-  forall g ys w,
-    gamma_recognize g ys w
-    -> exists v,
-      gamma_derivation g ys w v.
-Proof.
-  intros g ys w hg.
-  induction hg using gamma_recognize_mutual_ind with
-      (P := fun s w (hs : sym_recognize g s w) => 
-              exists t, sym_derivation g s w t); firstorder; eauto.
-  repeat econstructor; eauto.
-Qed.
+  (* Inductive definition of a nullable grammar symbol *)
+  Inductive nullable_sym (g : grammar) : symbol -> Prop :=
+  | NullableSym : forall x ys,
+      In (x, ys) g
+      -> nullable_gamma g ys
+      -> nullable_sym g (NT x)
+  with nullable_gamma (g : grammar) : list symbol -> Prop :=
+       | NullableNil  : nullable_gamma g []
+       | NullableCons : forall hd tl,
+           nullable_sym g hd
+           -> nullable_gamma g tl
+           -> nullable_gamma g (hd :: tl).
 
-(* Inductive definition of a nullable grammar symbol *)
-Inductive nullable_sym (g : grammar) : symbol -> Prop :=
-| NullableSym : forall x ys,
-    In (x, ys) g
-    -> nullable_gamma g ys
-    -> nullable_sym g (NT x)
-with nullable_gamma (g : grammar) : list symbol -> Prop :=
-     | NullableNil  : nullable_gamma g []
-     | NullableCons : forall hd tl,
-         nullable_sym g hd
-         -> nullable_gamma g tl
-         -> nullable_gamma g (hd :: tl).
+  Hint Constructors nullable_sym nullable_gamma.
 
-Hint Constructors nullable_sym nullable_gamma.
+  Lemma nullable_split :
+    forall g xs ys,
+      nullable_gamma g (xs ++ ys)
+      -> nullable_gamma g xs /\ nullable_gamma g ys.
+  Proof.
+    intros g xs; induction xs as [| x xs IH]; intros ys hn; sis; auto.
+    inv hn; firstorder.
+  Qed.
 
-Lemma nullable_split :
-  forall g xs ys,
-    nullable_gamma g (xs ++ ys)
-    -> nullable_gamma g xs /\ nullable_gamma g ys.
-Proof.
-  intros g xs; induction xs as [| x xs IH]; intros ys hn; sis; auto.
-  inv hn; firstorder.
-Qed.
+  Lemma nullable_split_l :
+    forall g xs ys,
+      nullable_gamma g (xs ++ ys)
+      -> nullable_gamma g ys.
+  Proof.
+    intros g xs ys hn; apply nullable_split in hn; firstorder.
+  Qed.
 
-Lemma nullable_split_l :
-  forall g xs ys,
-    nullable_gamma g (xs ++ ys)
-    -> nullable_gamma g ys.
-Proof.
-  intros g xs ys hn; apply nullable_split in hn; firstorder.
-Qed.
+  Lemma nullable_app :
+    forall g xs ys,
+      nullable_gamma g xs
+      -> nullable_gamma g ys
+      -> nullable_gamma g (xs ++ ys).
+  Proof.
+    intros g xs ys hng hng'.
+    induction xs as [| x xs]; sis; inv hng; auto.
+  Qed.
 
-Lemma nullable_app :
-  forall g xs ys,
-    nullable_gamma g xs
-    -> nullable_gamma g ys
-    -> nullable_gamma g (xs ++ ys).
-Proof.
-  intros g xs ys hng hng'.
-  induction xs as [| x xs]; sis; inv hng; auto.
-Qed.
+  Inductive nullable_path (g : grammar) :
+    symbol -> symbol -> Prop :=
+  | DirectPath : forall x z gamma pre suf,
+      In (x, gamma) g
+      -> gamma = pre ++ NT z :: suf
+      -> nullable_gamma g pre
+      -> nullable_path g (NT x) (NT z)
+  | IndirectPath : forall x y z gamma pre suf,
+      In (x, gamma) g
+      -> gamma = pre ++ NT y :: suf
+      -> nullable_gamma g pre
+      -> nullable_path g (NT y) (NT z)
+      -> nullable_path g (NT x) (NT z).
 
-Inductive nullable_path (g : grammar) :
-  symbol -> symbol -> Prop :=
-| DirectPath : forall x z gamma pre suf,
-    In (x, gamma) g
-    -> gamma = pre ++ NT z :: suf
-    -> nullable_gamma g pre
-    -> nullable_path g (NT x) (NT z)
-| IndirectPath : forall x y z gamma pre suf,
-    In (x, gamma) g
-    -> gamma = pre ++ NT y :: suf
-    -> nullable_gamma g pre
-    -> nullable_path g (NT y) (NT z)
-    -> nullable_path g (NT x) (NT z).
+  Hint Constructors nullable_path.
 
-Hint Constructors nullable_path.
+  Lemma nullable_path_trans :
+    forall g x y z,
+      nullable_path g x y
+      -> nullable_path g y z
+      -> nullable_path g x z.
+  Proof.
+    intros g x y z hxy hyz.
+    induction hxy; sis; subst.
+    - destruct z as [a | z]; eauto.
+      inv hyz.
+    - destruct z as [a | z]; eauto.
+      inv hyz.
+  Qed.  
 
-Lemma nullable_path_trans :
-  forall g x y z,
-    nullable_path g x y
-    -> nullable_path g y z
-    -> nullable_path g x z.
-Proof.
-  intros g x y z hxy hyz.
-  induction hxy; sis; subst.
-  - destruct z as [a | z]; eauto.
-    inv hyz.
-  - destruct z as [a | z]; eauto.
-    inv hyz.
-Qed.  
+  Definition left_recursive g sym :=
+    nullable_path g sym sym.
 
-Definition left_recursive g sym :=
-  nullable_path g sym sym.
+  Definition no_left_recursion g :=
+    forall (x : nonterminal), 
+      ~ left_recursive g (NT x).
 
-Definition no_left_recursion g :=
-  forall (x : nonterminal), 
-    ~ left_recursive g (NT x).
+End DefsFn.
 
+Module Type DefsT (SymTy : SYMBOL_TYPES).
+  Include DefsFn SymTy.
+End DefsT.
+
+Module Type T.
+  Declare Module SymTy : SYMBOL_TYPES.
+  Declare Module Defs  : DefsT SymTy.
+  Export SymTy.
+  Export Defs.
+End T.
